<?xml version="1.0" encoding="UTF-8"?>

<handout xml:id="week1-handout">
<title>Week 1 Handout: Laplace Transform </title>

<page>
  <paragraphs>
    <definition xml:id="def-laplace">
      <statement>
        <p> If <m>f</m> is a function defined for <m> t\geq 0</m>, then the integral 
          <m>\mathscr{L}\{f(t)\}=\int_0^\infty e^{-st}f(t)dt</m> is the <term>Laplace transform </term> of <m> f, </m>
          provided the integral converges. </p>

          <p> Sufficient conditions for existence:
            <ul>
              <li>
                <p> <m>f</m> must be piecewise continuous on <m>[0,\infty]</m>             
                </p>
              </li>
              <li>
                <p><m>f</m> must be of exponential order for <m>t > T</m>
                </p>
              </li>
            </ul>
          </p>
      </statement>
    </definition>


    <remark> 
      <p>
        <m>\mathscr{L}</m> is a linear transform, i.e.,
        <m> \mathscr{L}\{\alpha f(t)+ \beta g(t)\}=\alpha\mathscr{L}\{f(t)\}+\beta\mathscr{L}\{g(t)\}.</m>
      </p>
    </remark> 

    <example>
    <statement>
      <p>    <ol>
      <li>
        <p>Evaluate <m> \mathscr{L}\{t\}.</m>      
        </p> 
      </li>
      <li>
        <p> Evaluate  <m>\mathscr{L}\{f(t)\},</m>       
          where <m>   f(t) = \begin{cases}   0, &amp; 0\leq t\lt 3 \\  2, &amp; t\geq 3 \end{cases}  </m>
          <figure xml:id="fig-piecewise-graph">
            <caption>Graph of a piecewise function</caption>
            <image xml:id="graph-piecewise" width="60%">
            <shortdescription>The graph of a piecewise function with two horizontal segments. From t equals 0 to t equals 3, 
              the graph is on the t-axis at y equals 0, ending with an open circle 
              at (3, 0). For t greater than or equal to 3, the graph is a horizontal 
              line at y equals 2, starting with a closed circle at (3, 2).</shortdescription>
            <latex-image>
              \begin{tikzpicture}
                \begin{axis}[
                  axis x line=middle,
                  axis y line=middle,
                  xlabel={$t$},
                  ylabel={$y$},
                  ymin=-0.5, ymax=2.5,
                  xmin=0, xmax=5
                  ]
                  <!-- First piece: y = 0 for x < 3 -->
                  \addplot[domain=0:3, blue, thick] {0};
          
                  <!-- Second piece: y = 2 for x >= 2 -->
                  \addplot[domain=3:5, red, thick] {2};

                  <!-- Optional: Add open/closed circles for continuity -->
                  \draw[blue, fill=white] (axis cs:3,0) circle (2pt); <!-- open circle --> 
                  \draw[red, fill=red] (axis cs:3,2) circle (2pt); <!-- close circle -->
                \end{axis}
              \end{tikzpicture}
            </latex-image>
          </image>
        </figure>
        </p>
      </li>
    </ol>          
    </p>
    </statement>    
    <solution>
      <p> 
        <ol>
          <li>
            <p>
              <m> \mathscr{L}\{t\}=\int_0^\infty t e^{-st}dt=\left.-\frac{-te^{-st}}{s}\right|_0^{\infty}+\frac{1}{s}\int_0^\infty e^{-st}dt=\frac{1}{s^2}</m>
            </p>
          </li>
          <li>
            <p>
              <m>\mathscr{L}\{f(t)\}=\int_0^3e^{-st}\cdot 0dt+\int_3^\infty e^{-st}\cdot 2 dt=\frac{2e^{-3s}}{s}, s>0</m>
            </p>
          </li>
        </ol>
        
      </p>
    </solution>
    </example>


    
  </paragraphs>
</page>
<page>
  <p>
    <definition xml:id="def-laplace-inverse">
      <statement>
        <p> If <m>F(s)</m> represents the Laplace transform of a function <m>f(t),</m>
          then <m>f(t)</m> is the <term>inverse Laplace transform</term> of <m>F(s),</m>
          <md>             f(t)=\mathscr{L}^{-1}\left\{F(s)\right\} </md>
        </p>

        <p>
          <m>\mathscr{L}^{-1}</m> is a linear transform,
          <md>\mathscr{L}^{-1}\left\{\alpha F(s)+\beta G(s)\right\}
          =\alpha\mathscr{L}^{-1}\left\{F(s)\right\}+\beta G(s)\mathscr{L}^{-1}\left\{G(s)\right\}</md>
        </p>
      </statement>
    </definition>
  </p>
  <theorem xml:id="thm-laplace-inverse">
    <statement>
      <p><ol>
        <li> <p> <m>1=\mathscr{L}^{-1}\left\{\frac{1}{s}\right\}</m> </p> </li>
        <li> <p> <m>t^n=\mathscr{L}^{-1}\left\{\frac{n!}{s^{n+1}}\right\}, n=1,2,3,\ldots</m> </p></li>
        <li> <p> <m>e^{at}=\mathscr{L}^{-1}\left\{\frac{1}{s-a}\right\}</m></p></li>
        <li> <p> <m>\sin kt=\mathscr{L}^{-1}\left\{\frac{k}{s^2+k^2}\right\}</m></p></li>
        <li> <p> <m>\cos kt=\mathscr{L}^{-1}\left\{\frac{s}{s^2+k^2}\right\}</m></p></li>
        <li> <p> <m>\sinh kt=\mathscr{L}^{-1}\left\{\frac{k}{s^2-k^2}\right\}</m></p> </li>
        <li> <p> <m>\cosh kt=\mathscr{L}^{-1}\left\{\frac{s}{s^2-k^2}\right\}</m>  </p> </li>
      </ol>
        
      </p>
    </statement> 
  </theorem>
  
  <example>
    <statement> Use Theorem <xref ref="thm-laplace-inverse"/> to find each of the followings:
    <ol>
      <li> <p> <m>\mathscr{L}^{-1}\left\{\frac{1}{s^4}\right\}</m></p> </li>
      <li> <p> <m>\mathscr{L}^{-1}\left\{\frac{5s}{s^2+6}\right\}</m> </p> </li>
    </ol>
    </statement>
    <solution>
      <p> <ol>
        <li> <p>   Using (b) in Theorem <xref ref="thm-laplace-inverse"/>,<m>n</m> should be 3. Thus 
        <md>\frac{1}{s^4}=\frac{1}{3!}\cdot\frac{3!}{s^{3+1}}\Rightarrow \mathscr{L}^{-1}\left\{\frac{1}{s^4}\right\}=
          \frac{1}{3!}\mathscr{L}^{-1}\left\{\frac{3!}{s^{3+1}}\right\}=\frac{1}{3!}t^3.</md>  </p>  </li>
        <li> <p>   Using (e) in Theorem <xref ref="thm-laplace-inverse"/>, <m>k</m> is <m>\sqrt{6}.</m>  Thus
        <md> \mathscr{L}^{-1}\left\{\frac{5s}{s^2+6}\right\}=5\mathscr{L}^{-1}\left\{\frac{s}{s^2+\sqrt{6}^2}\right\}
          =5\cos\sqrt{6}t </md> </p> </li>
      </ol>
        
      </p>
    </solution>
  </example>
  <example> <statement>
    <p> Find <m>\mathscr{L}^{-1}\left\{\dfrac{2s+8}{s^2-9}\right\}.</m> </p>
  </statement> 
  <solution> <p> <m>\frac{2s+8}{s^2-9}</m> can be written into two expressions:
    <ul>
      <li> <p> <m>\frac{2s+8}{s^2-9}=\frac{2s}{s^2-9}+\frac{8}{s^2-9} </m> 
        <md>\Rightarrow \mathscr{L}^{-1}\left\{\dfrac{2s+8}{s^2-9}\right\}=2\cosh 3t+\frac{8}{3}\sinh 3t </md>  </p>  </li>
      <li> <p> <m> \frac{2s+8}{s^2-9}=\frac{2(s+3)}{s^2-9}+\frac{2}{s^2-9}=\frac{2}{s-3}+\frac{2}{s^2-9}</m>
      <md>\Rightarrow \mathscr{L}^{-1}\left\{\dfrac{2s+8}{s^2-9}\right\}= 2e^{3t}+\frac{2}{3}\sinh 3t</md></p> </li>   
      
      </ul>  
    </p>
  </solution>  
  </example>
</page>

</handout>
